Test/og/runtest.bat
@@ -3,13 +3,13 @@ setlocal
 
 set BGEXE=..\..\Binaries\Boogie.exe
 
-for %%f in (foo.bpl bar.bpl one.bpl parallel1.bpl parallel3.bpl) do (
+for %%f in (foo.bpl bar.bpl one.bpl parallel1.bpl) do (
   echo.
   echo -------------------- %%f --------------------
   %BGEXE% %* /nologo /noinfer %%f
 )
 
-for %%f in (linear-set.bpl linear-set2.bpl FlanaganQadeer.bpl DeviceCacheSimplified.bpl parallel2.bpl parallel4.bpl parallel5.bpl parallel6.bpl parallel7.bpl akash.bpl t1.bpl new1.bpl perm.bpl async.bpl) do (
+for %%f in (linear-set.bpl linear-set2.bpl FlanaganQadeer.bpl DeviceCacheSimplified.bpl parallel2.bpl parallel4.bpl parallel5.bpl akash.bpl t1.bpl new1.bpl perm.bpl async.bpl) do (
   echo.
   echo -------------------- %%f --------------------
   %BGEXE% %* /nologo /noinfer /typeEncoding:m /useArrayTheory %%f
